fix up admits in dot product

src/lib/poly/Kuiper.Poly.DotProduct.fst
@@ -135,19 +135,57 @@ fn setup
     (forall+ (bid : natlt lena). kpre lena ga1 ga2 s1 s2 vr1 vr2 bid) **
     emp (* frame *)
 {
-  // mk_mbarrier nthr (HR.barrier_matrix nthr ar (pmul s1 s2));
   mk_mbarrier lena (HR.barrier_matrix lena ga1 (pmul s1 s2) (rsmul vr1 vr2));
+  gpu_array_slice_1 ga2;
+  forevery_zip 
+    (fun (i: natlt (v lena)) -> gpu_pts_to_slice ga2 i (i + 1) seq![Seq.Base.index s2 i]) _;
   gpu_array_slice_1 ga1;
-  // bigstar_zip 0 lena _ _;
-  // gpu_array_slice_1 ga2;
-  // bigstar_zip 0 lena _ _;
-  // slice
-  // bigstar_zip 0 nthr (gpu_pts_to_array1 ar) (mbarrier_tok nthr (HR.barrier_matrix nthr ar (pmul s1 s2)) 0);
-  // rewrite each nthr as Enumerable.cardinal (natlt nthr) #_;
-  // forevery_fromstar #(natlt nthr) (fun i ->
-  //   gpu_pts_to_array1 ar i **
-  //   mbarrier_tok nthr (HR.barrier_matrix nthr ar (pmul s1 s2)) 0 i);
-  admit()
+  forevery_zip (fun (i: natlt (v lena)) -> gpu_pts_to_slice ga1 i (i + 1) seq![Seq.Base.index s1 i]) _;
+  forevery_map 
+   (fun (i: natlt (v lena)) -> //too bad that you have to write this; inference should find it
+      gpu_pts_to_slice ga1 i (i + 1) seq![Seq.Base.index s1 i] **
+      gpu_pts_to_slice ga2 i (i + 1) seq![Seq.Base.index s2 i] **
+      mbarrier_tok lena (HR.barrier_matrix lena ga1 (pmul s1 s2) (rsmul vr1 vr2)) 0 i)
+   (kpre lena ga1 ga2 s1 s2 vr1 vr2) fn bid { fold kpre lena ga1 ga2 s1 s2 vr1 vr2 bid };
+}
+
+ghost
+fn teardown
+  (#et:Type0) {| scalar et, real_like et |}
+  (lena : szp{SZ.v lena <= max_threads})
+  (ga1 ga2 : gpu_array et lena)
+  (#s1 #s2 : seq et)
+  (#vr1 #vr2 : seq real { seq_approximates s1 vr1 /\ seq_approximates s2 vr2 })
+  (_: squash ( len s1 == SZ.v lena /\ len s2 == SZ.v lena ))
+  norewrite
+  requires
+    (forall+ (tid : natlt lena). kpost lena ga1 ga2 s1 s2 vr1 vr2 tid) **
+    emp
+  ensures
+    ga2 |-> s2 ** 
+    (exists* (s1' : seq et{Seq.length s1' > 0}). 
+      (ga1 |-> s1') **
+      pure ((s1' @! 0) `approximates` real_seq_sum (rsmul vr1 vr2)))
+{ 
+  // rewrite_by (forall+ (tid : natlt lena). kpost lena ga1 ga2 s1 s2 vr1 vr2 tid) _ 
+  //            (slprop_equiv_unfold (`%kpost)) ();
+  //  rewrite (forall+ (tid : natlt lena). kpost lena ga1 ga2 s1 s2 vr1 vr2 tid) as _ by (norm [delta_only [`kpost]]);
+  forevery_map (kpost lena ga1 ga2 s1 s2 vr1 vr2)
+    (fun tid ->
+      gpu_pts_to_slice ga2 tid (tid + 1) seq![s2 @! tid] **
+      ((exists* it.
+        mbarrier_tok lena (HR.barrier_matrix lena ga1 (pmul s1 s2) (rsmul vr1 vr2)) it tid) **
+       (if_ (tid = 0) (HR.gpu_pts_to_slice_sum ga1 0 lena (pmul s1 s2) (rsmul vr1 vr2)))))
+    fn tid { unfold (kpost lena ga1 ga2 s1 s2 vr1 vr2 tid) };
+  forevery_unzip _ _;
+  gpu_array_unslice_1 ga2;
+  forevery_unzip _ _;
+  forevery_extract #(natlt lena) 0 
+    (fun tid -> (if_ (tid = 0) (HR.gpu_pts_to_slice_sum ga1 0 lena (pmul s1 s2) (rsmul vr1 vr2))));
+  if_elim_true _;
+  drop_ (Pulse.Lib.Trade.trade _ _);
+  drop_ (forall+ (tid:natlt lena). _);
+  unfold HR.gpu_pts_to_slice_sum ga1 0 lena (pmul s1 s2) (rsmul vr1 vr2);
 }
 
 inline_for_extraction noextract
@@ -167,13 +205,14 @@ let dp_kernel
     f = kf lena ga1 ga2 #s1 #s2;
 
     block_setup    = setup lena ga1 ga2 #s1 #s2;
-    block_teardown = magic ();
+    block_teardown = teardown lena ga1 ga2 #s1 #s2;
 
     kpre  = kpre lena ga1 ga2 s1 s2 vr1 vr2;
     kpost = kpost lena ga1 ga2 s1 s2 vr1 vr2;
 
     frame = emp;
   } <: kernel_desc_1_n _ _
+
 
 inline_for_extraction noextract
 fn dotprod
@@ -193,7 +232,7 @@ fn dotprod
   returns
     dp: et
   ensures
-    pure (dp == sum (pmul v1 v2))
+    pure (dp `approximates` sum (pmul vr1 vr2))
 {
   Pulse.Lib.Vec.pts_to_len a1;
   Pulse.Lib.Vec.pts_to_len a2;
@@ -217,7 +256,9 @@ fn dotprod
   (* swap space *)
   let ar = V.alloc #et zero 1sz;
   (* inference sucks here, what's going on? *)
-  Kuiper.Array.gpu_memcpy_device_to_host' #_ #_ #1 ar 0sz #_ ga1 0sz 1sz;
+  Kuiper.Array.gpu_memcpy_device_to_host' #_ #_ #1 //the dst_sz cannot be computed by unification; 
+      ar 0sz //#_
+      ga1 0sz 1sz;
 
   gpu_array_free ga1;
   gpu_array_free ga2;
@@ -226,9 +267,7 @@ fn dotprod
   V.free ar;
 
   (* Finally, ensure that the reduction must be sum *)
-  assume (pure (dp == sum (pmul v1 v2)));
-  // fixme: should come from approximation now
-  // Kuiper.IsReduction.ac_eq_foldl zero add (pmul v1 v2) dp;
+  assert pure (rsmul vr1 vr2 `Seq.equal` pmul vr1 vr2);
 
   dp
 }
